Flapjack/Tests.lean
@@ -68,6 +68,7 @@ import Flapjack.Test.StaticStructFieldsParity
 import Flapjack.Test.StaticShapeParity
 import Flapjack.Test.StaticIdShapesParity
 import Flapjack.Test.StaticExpParity
+import Flapjack.Test.StaticProgParity
 import Flapjack.Test.CorrectnessConditional
 import Flapjack.Test.CorrectnessColour
 import Flapjack.Test.CorrectnessSsaColour
